\documentclass[12pt,a4paper]{article}
\usepackage[utf8]{inputenc}
\usepackage[english]{babel}
\usepackage[fleqn]{amsmath}
\usepackage{nccmath}
\usepackage{amsfonts}
\usepackage{amssymb}
\usepackage{graphicx}
\usepackage[left=2cm,right=2cm,top=2cm,bottom=2cm]{geometry}
\author{Henry Yu}
\title{A6N4 Writeup}
\setlength{\mathindent}{0pt}
\begin{document}

\begin{titlepage}
	
	\begin{center}

		\vspace*{\fill}

    	\vspace*{0.5cm}
	
	    \huge{Perfect Writeup: Assignment 6 No. 4}
	
	    \vspace*{0.5cm}
	
	    \large{Henry Yu}
	
    	\vspace*{\fill}

	\end{center}

\end{titlepage}

\newpage

\raggedright

\underline{Question 4}

\bigbreak


Verify that for any two three-dimensional vectors $\vec{u}$ and $\vec{v}$,
\begin{ceqn}
\begin{align*}
(|\vec{u} \times \vec{v}|)^{2}+(\vec{u} \cdot \vec{v})^{2}=(|\vec{u}||\vec{v}|)^{2}
\end{align*}
\end{ceqn}
i.e.,
\begin{ceqn}
\begin{align*}
\left(\frac{|\vec{u} \times \vec{v}|}{|\vec{u}||\vec{v}|}\right)^{2}+\left(\frac{\vec{u} \cdot \vec{v}}{|\vec{u}||\vec{v}|}\right)^{2}=1.
\end{align*}
\end{ceqn}

What is the trigonometric relevance of this fact?

\vspace{1cm}

Note that,
\begin{align*}
	&(|\vec{u} \times \vec{v}|)^{2}+(\vec{u} \cdot \vec{v})^{2}=\,(|\vec{u}||\vec{v}|)^{2}  \\
	&=\,(u_1^{2}+u_2^{2}+u_3^{2})(v_1^{2}+v_2^{2}+v_3^{2}). \\
\end{align*}

\vspace{-10pt}

Thus,
\begin{align*}
	(|\vec{u} \times \vec{v}|)^{2}&=\,|\vec{u}|^{2}|\vec{v}|^{2}-|\vec{u}|^{2}|\vec{v}|^{2}\,\cos\,\theta \\
	&=\,|\vec{u}|^{2}|\vec{v}|^{2}(1-\cos\,\theta)\,\sin^{2}\,\theta.
\end{align*}

Thus,
\begin{align*}
(|\vec{u} \times \vec{v}|)=(|\vec{u}||\vec{v}|)\,\sin\,\theta.
\end{align*}

$\therefore$
\begin{align*}
    \sin\,\theta=\left(\frac{|\vec{u} \times \vec{v}|}{|\vec{u}||\vec{v}|}\right).
\end{align*}

\begin{center}
\rule{8cm}{0.4pt}
\end{center}

Note that,
\begin{align*}
    |\vec{u}-\vec{v}|^{2}=|\vec{u}|^{2}+|\vec{v}|^{2}-2|\vec{u}||\vec{v}|\cos\,\theta.
\end{align*}

Thus,
\begin{align*}
    2|\vec{u}||\vec{v}|\cos\,\theta&=|\vec{u}|^{2}+|\vec{v}|^{2}-|\vec{u}-\vec{v}|^{2} \\
    &=(u_1^{2}+u_2^{2}+u_3^{2})+(v_1^{2}+v_2^{2}+v_3^{2})-(u_1-v_1)^{2}-(u_2-v_2)^{2}-(u_3-v_3)^{2} \\
    &=u_1^{2}+u_2^{2}+u_3^{2}+v_1^{2}+v_2^{2}+v_3^{2}-(u_1^{2}-2u_1v_1+v_1^{2})-(u_2^{2}-2u_2v_2+v_2^{2})-(u_3^{2}-2u_3v_3+v_3^{2}) \\
    &=2u_1v_1+2u_2v_2+2u_3v_3 \\
    |\vec{u}||\vec{v}|\cos\,\theta&=u_1v_1+u_2v_2+u_3v_3
\end{align*}

$\therefore$
\begin{align*}
    \cos\,\theta=\left(\frac{\vec{u} \cdot \vec{v}}{|\vec{u}||\vec{v}|}\right).
\end{align*}

\begin{center}
\rule{8cm}{0.4pt}
\end{center}

\begin{ceqn}
    \begin{align*}
        \left(\frac{|\vec{u} \times \vec{v}|}{|\vec{u}||\vec{v}|}\right)^{2}+\left(\frac{\vec{u} \cdot \vec{v}}{|\vec{u}||\vec{v}|}\right)^{2}=1.
    \end{align*}
\end{ceqn}

\begin{ceqn}
    \begin{align*}
        (\cos\,\theta)\,^2+(\sin\,\theta)\,^2=1.
    \end{align*}
\end{ceqn}
\end{document}